use state instead of set of heap locations for well-definedness check; add candidate for unfolding semantics

TotalExpressions.thy
@@ -78,40 +78,53 @@ fun sub_expressions_atomic :: "pure_exp atomic_assert \<Rightarrow> pure_exp set
 text\<open>Pure expression evaluation, where the set of heap locations expresses the set of readable locations
 (if no set is provided, then all locations can be read).
 \<close>
-inductive red_pure_exp_total :: "program \<Rightarrow> 'a interp \<Rightarrow> heap_loc set \<Rightarrow> pure_exp \<Rightarrow> 'a full_total_state \<Rightarrow> 'a extended_val \<Rightarrow> bool"
+inductive red_pure_exp_total :: "program \<Rightarrow> 'a interp \<Rightarrow> 'a full_total_state option \<Rightarrow> pure_exp \<Rightarrow> 'a full_total_state \<Rightarrow> 'a extended_val \<Rightarrow> bool"
   ("_, _, _ \<turnstile> ((\<langle>_;_\<rangle>) [\<Down>]\<^sub>t _)" [51,51,51,0,51,51] 81) and
-   red_pure_exps_total :: "program \<Rightarrow> 'a interp \<Rightarrow> heap_loc set \<Rightarrow> pure_exp list \<Rightarrow> 'a full_total_state \<Rightarrow> (('a val) list) option \<Rightarrow> bool" and
-   red_inhale :: "program \<Rightarrow>  'a interp \<Rightarrow> ('a full_total_state \<Rightarrow> bool) \<Rightarrow> assertion \<Rightarrow> 'a full_total_state \<Rightarrow> 'a standard_result \<Rightarrow> bool"
+   red_pure_exps_total :: "program \<Rightarrow> 'a interp \<Rightarrow> 'a full_total_state option \<Rightarrow> pure_exp list \<Rightarrow> 'a full_total_state \<Rightarrow> (('a val) list) option \<Rightarrow> bool" and
+   red_inhale :: "program \<Rightarrow>  'a interp \<Rightarrow> ('a full_total_state \<Rightarrow> bool) \<Rightarrow> assertion \<Rightarrow> 'a full_total_state \<Rightarrow> 'a standard_result \<Rightarrow> bool" and
+   unfold_rel :: "program \<Rightarrow> 'a interp \<Rightarrow> predicate_ident \<Rightarrow> ('a val list) \<Rightarrow> prat \<Rightarrow> 'a full_total_state \<Rightarrow> 'a full_total_state \<Rightarrow> bool"
   for Pr :: program and \<Delta> :: "'a interp"
   where
+\<comment>\<open>unfold_rel\<close>
+  UnfoldRelStep: 
+    "\<lbrakk> ViperLang.predicates Pr pred_id = Some pred_decl;
+     ViperLang.predicate_decl.body pred_decl = Some pred_body;
+     m = get_mp_total_full \<omega>;
+     pgte (m (pred_id,vs)) q;
+     q \<noteq> pnone;
+     m' = m( (pred_id,vs) := psub (m (pred_id, vs)) q);
+     \<omega>2 = (nth_option vs, get_trace_total \<omega>, update_mp_total (get_total_full \<omega>) m');
+     red_inhale Pr \<Delta> (\<lambda>_. True) (syntactic_mult (Rep_prat q) pred_body) \<omega>2 (RNormal \<omega>') \<rbrakk> \<Longrightarrow> 
+     unfold_rel Pr \<Delta> pred_id vs q \<omega> \<omega>'"
+
 \<comment>\<open>Atomic inhale\<close>
-  InhAcc: 
-    "\<lbrakk> Pr, \<Delta>, get_valid_locs \<omega> \<turnstile> \<langle>e_r; \<omega>\<rangle> [\<Down>]\<^sub>t Val (VRef r); 
-       Pr, \<Delta>, get_valid_locs \<omega> \<turnstile> \<langle>e_p; \<omega>\<rangle> [\<Down>]\<^sub>t Val (VPerm p); 
+| InhAcc: 
+    "\<lbrakk> Pr, \<Delta>, Some \<omega> \<turnstile> \<langle>e_r; \<omega>\<rangle> [\<Down>]\<^sub>t Val (VRef r); 
+       Pr, \<Delta>, Some \<omega> \<turnstile> \<langle>e_p; \<omega>\<rangle> [\<Down>]\<^sub>t Val (VPerm p); 
        W' = inhale_perm_single R \<omega> (the_address r,f) (Some (Abs_prat p));
        th_result_rel (p \<ge> 0) (W' \<noteq> {} \<and> r \<noteq> Null) W' res \<rbrakk> \<Longrightarrow>
        red_inhale Pr \<Delta> R (Atomic (Acc e_r f (PureExp e_p))) \<omega> res"
 | InhAccPred:
-    "\<lbrakk> Pr, \<Delta>, get_valid_locs \<omega> \<turnstile> \<langle>e_p; \<omega>\<rangle> [\<Down>]\<^sub>t Val (VPerm p);
-       red_pure_exps_total Pr \<Delta> (get_valid_locs \<omega>) e_args \<omega> (Some v_args);
+    "\<lbrakk> Pr, \<Delta>, Some \<omega> \<turnstile> \<langle>e_p; \<omega>\<rangle> [\<Down>]\<^sub>t Val (VPerm p);
+       red_pure_exps_total Pr \<Delta> (Some \<omega>) e_args \<omega> (Some v_args);
        W' = inhale_perm_single_pred R \<omega> (pred_id, v_args) (Some (Abs_prat p));
        th_result_rel (p \<ge> 0) (W' \<noteq> {}) W' res \<rbrakk> \<Longrightarrow>       
        red_inhale Pr \<Delta> R (Atomic (AccPredicate pred_id e_args (PureExp e_p))) \<omega> res"
 | InhAccWildcard: 
-    "\<lbrakk> Pr, \<Delta>, get_valid_locs \<omega> \<turnstile> \<langle>e_r; \<omega>\<rangle> [\<Down>]\<^sub>t Val (VRef r);
+    "\<lbrakk> Pr, \<Delta>, Some \<omega> \<turnstile> \<langle>e_r; \<omega>\<rangle> [\<Down>]\<^sub>t Val (VRef r);
        W' = inhale_perm_single R \<omega> (the_address r,f) None;
        th_result_rel True (W' \<noteq> {} \<and> r \<noteq> Null) W' res \<rbrakk> \<Longrightarrow>
        red_inhale Pr \<Delta> R (Atomic (Acc e_r f Wildcard)) \<omega> res"
 | InhAccPredWildcard: 
-    "\<lbrakk> red_pure_exps_total Pr \<Delta> (get_valid_locs \<omega>) e_args \<omega> (Some v_args);
+    "\<lbrakk> red_pure_exps_total Pr \<Delta> (Some \<omega>) e_args \<omega> (Some v_args);
        W' = inhale_perm_single_pred R \<omega> (pred_id, v_args) None;
        th_result_rel True (W' \<noteq> {}) W' res \<rbrakk> \<Longrightarrow>
        red_inhale Pr \<Delta> R (Atomic (AccPredicate pred_id e_args Wildcard)) \<omega> res"
 | InhPureNormalMagic: 
-    "\<lbrakk> Pr, \<Delta>, get_valid_locs \<omega> \<turnstile> \<langle>e; \<omega>\<rangle> [\<Down>]\<^sub>t Val (VBool b) \<rbrakk> \<Longrightarrow>
+    "\<lbrakk> Pr, \<Delta>, Some \<omega> \<turnstile> \<langle>e; \<omega>\<rangle> [\<Down>]\<^sub>t Val (VBool b) \<rbrakk> \<Longrightarrow>
       red_inhale Pr \<Delta> R (Atomic (Pure e)) \<omega> (if b then RNormal \<omega> else RMagic)"
 | InhSubFailure: 
-    "\<lbrakk> e \<in> sub_expressions_atomic A; Pr, \<Delta>, get_valid_locs \<omega> \<turnstile> \<langle>e; \<omega>\<rangle> [\<Down>]\<^sub>t VFailure \<rbrakk> \<Longrightarrow> 
+    "\<lbrakk> e \<in> sub_expressions_atomic A; Pr, \<Delta>, Some \<omega> \<turnstile> \<langle>e; \<omega>\<rangle> [\<Down>]\<^sub>t VFailure \<rbrakk> \<Longrightarrow> 
       red_inhale Pr \<Delta> R (Atomic A) \<omega> RFailure"
 
 \<comment>\<open>Connectives inhale\<close>
@@ -125,14 +138,14 @@ inductive red_pure_exp_total :: "program \<Rightarrow> 'a interp \<Rightarrow> h
       red_inhale Pr \<Delta> R (A && B) \<omega> resA"
 | InhImpTrue:
  "\<lbrakk> 
-    Pr, \<Delta>, get_valid_locs \<omega> \<turnstile> \<langle>e; \<omega>\<rangle> [\<Down>]\<^sub>t (Val (VBool True)); 
+    Pr, \<Delta>, Some \<omega> \<turnstile> \<langle>e; \<omega>\<rangle> [\<Down>]\<^sub>t (Val (VBool True)); 
     red_inhale Pr \<Delta> R A \<omega> res \<rbrakk> \<Longrightarrow>
     red_inhale Pr \<Delta> R (Imp e A) \<omega> res"
 | InhImpFalse:
- "\<lbrakk> Pr, \<Delta>, get_valid_locs \<omega> \<turnstile> \<langle>e; \<omega>\<rangle> [\<Down>]\<^sub>t Val (VBool False) \<rbrakk> \<Longrightarrow> 
+ "\<lbrakk> Pr, \<Delta>, Some \<omega> \<turnstile> \<langle>e; \<omega>\<rangle> [\<Down>]\<^sub>t Val (VBool False) \<rbrakk> \<Longrightarrow> 
     red_inhale Pr \<Delta> R (Imp e A) \<omega> (RNormal \<omega>)"
 | InhImpFailure:
- "\<lbrakk> Pr, \<Delta>, get_valid_locs \<omega> \<turnstile> \<langle>e; \<omega>\<rangle> [\<Down>]\<^sub>t VFailure \<rbrakk> \<Longrightarrow>
+ "\<lbrakk> Pr, \<Delta>, Some \<omega> \<turnstile> \<langle>e; \<omega>\<rangle> [\<Down>]\<^sub>t VFailure \<rbrakk> \<Longrightarrow>
    red_inhale Pr \<Delta> R (Imp e A) \<omega> RFailure"
 
 \<comment>\<open>Pure expression evaluation\<close>
@@ -146,48 +159,55 @@ inductive red_pure_exp_total :: "program \<Rightarrow> 'a interp \<Rightarrow> h
      red_pure_exps_total Pr \<Delta> LH es \<omega> None"
 
 \<comment>\<open>Atomic expressions\<close>
-| RedLit: "Pr, \<Delta>, LH \<turnstile> \<langle>ELit l; _\<rangle> [\<Down>]\<^sub>t Val (val_of_lit l)"
-| RedVar: "\<lbrakk> \<sigma> n = Some v \<rbrakk> \<Longrightarrow> Pr, \<Delta>, LH \<turnstile> \<langle>Var n; (\<sigma>, _, _)\<rangle> [\<Down>]\<^sub>t Val v"
-| RedResult: "\<lbrakk> \<sigma> 0 = Some v \<rbrakk> \<Longrightarrow> Pr, \<Delta>, LH \<turnstile> \<langle>Result; (\<sigma>, _, _)\<rangle> [\<Down>]\<^sub>t Val v"
+| RedLit: "Pr, \<Delta>, \<omega>_def \<turnstile> \<langle>ELit l; _\<rangle> [\<Down>]\<^sub>t Val (val_of_lit l)"
+| RedVar: "\<lbrakk> \<sigma> n = Some v \<rbrakk> \<Longrightarrow> Pr, \<Delta>, \<omega>_def \<turnstile> \<langle>Var n; (\<sigma>, _, _)\<rangle> [\<Down>]\<^sub>t Val v"
+| RedResult: "\<lbrakk> \<sigma> 0 = Some v \<rbrakk> \<Longrightarrow> Pr, \<Delta>, \<omega>_def \<turnstile> \<langle>Result; (\<sigma>, _, _)\<rangle> [\<Down>]\<^sub>t Val v"
 
 \<comment>\<open>Binop and Unop\<close>
-| RedBinopLazy: "\<lbrakk> Pr, \<Delta>, LH \<turnstile> \<langle>e1; \<omega>\<rangle> [\<Down>]\<^sub>t Val v1 ; eval_binop_lazy v1 bop = Some v \<rbrakk>
-  \<Longrightarrow> Pr, \<Delta>, LH \<turnstile> \<langle>Binop e1 bop e2; \<omega>\<rangle> [\<Down>]\<^sub>t Val v"
-| RedBinop: "\<lbrakk> Pr, \<Delta>, LH \<turnstile> \<langle>e1; \<omega>\<rangle> [\<Down>]\<^sub>t Val v1 ; Pr, \<Delta>, LH \<turnstile> \<langle>e2; \<omega>\<rangle> [\<Down>]\<^sub>t Val v2 ; eval_binop_lazy v1 bop = None; eval_binop v1 bop v2 = BinopNormal v \<rbrakk>
-  \<Longrightarrow> Pr, \<Delta>, LH \<turnstile> \<langle>Binop e1 bop e2; \<omega>\<rangle> [\<Down>]\<^sub>t Val v"
-| RedBinopRightFailure: "\<lbrakk> Pr, \<Delta>, LH \<turnstile> \<langle>e1; \<omega>\<rangle> [\<Down>]\<^sub>t Val v1; Pr, \<Delta>, LH \<turnstile> \<langle>e2; \<omega>\<rangle> [\<Down>]\<^sub>t VFailure;  eval_binop_lazy v1 bop = None \<rbrakk>
-  \<Longrightarrow> Pr, \<Delta>, LH \<turnstile> \<langle>Binop e1 bop e2; \<omega>\<rangle> [\<Down>]\<^sub>t VFailure"
-| RedBinopOpFailure: "\<lbrakk> Pr, \<Delta>, LH \<turnstile> \<langle>e1; \<omega>\<rangle> [\<Down>]\<^sub>t Val v1 ; Pr, \<Delta>, LH \<turnstile> \<langle>e2; \<omega>\<rangle> [\<Down>]\<^sub>t Val v2 ; eval_binop v1 bop v2 = BinopOpFailure ; eval_binop_lazy v1 bop = None \<rbrakk>
-  \<Longrightarrow> Pr, \<Delta>, LH \<turnstile> \<langle>Binop e1 bop e2; \<omega>\<rangle> [\<Down>]\<^sub>t VFailure" (* Division by 0 *)
-| RedBinopLeftFailure: "\<lbrakk> Pr, \<Delta>, LH \<turnstile> \<langle>e1; \<omega>\<rangle> [\<Down>]\<^sub>t VFailure \<rbrakk>
-  \<Longrightarrow> Pr, \<Delta>, LH \<turnstile> \<langle>Binop e1 bop e2; \<omega>\<rangle> [\<Down>]\<^sub>t VFailure" (* could be replaced *)
+| RedBinopLazy: "\<lbrakk> Pr, \<Delta>, \<omega>_def \<turnstile> \<langle>e1; \<omega>\<rangle> [\<Down>]\<^sub>t Val v1 ; eval_binop_lazy v1 bop = Some v \<rbrakk>
+  \<Longrightarrow> Pr, \<Delta>, \<omega>_def \<turnstile> \<langle>Binop e1 bop e2; \<omega>\<rangle> [\<Down>]\<^sub>t Val v"
+| RedBinop: "\<lbrakk> Pr, \<Delta>, \<omega>_def \<turnstile> \<langle>e1; \<omega>\<rangle> [\<Down>]\<^sub>t Val v1 ; Pr, \<Delta>, \<omega>_def \<turnstile> \<langle>e2; \<omega>\<rangle> [\<Down>]\<^sub>t Val v2 ; eval_binop_lazy v1 bop = None; eval_binop v1 bop v2 = BinopNormal v \<rbrakk>
+  \<Longrightarrow> Pr, \<Delta>, \<omega>_def \<turnstile> \<langle>Binop e1 bop e2; \<omega>\<rangle> [\<Down>]\<^sub>t Val v"
+| RedBinopRightFailure: "\<lbrakk> Pr, \<Delta>, \<omega>_def \<turnstile> \<langle>e1; \<omega>\<rangle> [\<Down>]\<^sub>t Val v1; Pr, \<Delta>, \<omega>_def \<turnstile> \<langle>e2; \<omega>\<rangle> [\<Down>]\<^sub>t VFailure;  eval_binop_lazy v1 bop = None \<rbrakk>
+  \<Longrightarrow> Pr, \<Delta>, \<omega>_def \<turnstile> \<langle>Binop e1 bop e2; \<omega>\<rangle> [\<Down>]\<^sub>t VFailure"
+| RedBinopOpFailure: "\<lbrakk> Pr, \<Delta>, \<omega>_def \<turnstile> \<langle>e1; \<omega>\<rangle> [\<Down>]\<^sub>t Val v1 ; Pr, \<Delta>, \<omega>_def \<turnstile> \<langle>e2; \<omega>\<rangle> [\<Down>]\<^sub>t Val v2 ; eval_binop v1 bop v2 = BinopOpFailure ; eval_binop_lazy v1 bop = None \<rbrakk>
+  \<Longrightarrow> Pr, \<Delta>, \<omega>_def \<turnstile> \<langle>Binop e1 bop e2; \<omega>\<rangle> [\<Down>]\<^sub>t VFailure" (* Division by 0 *)
+| RedBinopLeftFailure: "\<lbrakk> Pr, \<Delta>, \<omega>_def \<turnstile> \<langle>e1; \<omega>\<rangle> [\<Down>]\<^sub>t VFailure \<rbrakk>
+  \<Longrightarrow> Pr, \<Delta>, \<omega>_def \<turnstile> \<langle>Binop e1 bop e2; \<omega>\<rangle> [\<Down>]\<^sub>t VFailure" (* could be replaced *)
 
-| RedUnop: "\<lbrakk> Pr, \<Delta>, LH \<turnstile> \<langle>e; \<omega>\<rangle> [\<Down>]\<^sub>t Val v; eval_unop unop v = BinopNormal v' \<rbrakk> \<Longrightarrow> Pr, \<Delta>, LH \<turnstile> \<langle>Unop unop e; \<omega>\<rangle> [\<Down>]\<^sub>t Val v'"
-| RedUnopFailure: "\<lbrakk> Pr, \<Delta>, LH \<turnstile> \<langle>e; \<omega>\<rangle> [\<Down>]\<^sub>t VFailure \<rbrakk> \<Longrightarrow> Pr, \<Delta>, LH \<turnstile> \<langle>Unop unop e; \<omega>\<rangle> [\<Down>]\<^sub>t VFailure" (* could be replaced *)
+| RedUnop: "\<lbrakk> Pr, \<Delta>, \<omega>_def \<turnstile> \<langle>e; \<omega>\<rangle> [\<Down>]\<^sub>t Val v; eval_unop unop v = BinopNormal v' \<rbrakk> \<Longrightarrow> Pr, \<Delta>, \<omega>_def \<turnstile> \<langle>Unop unop e; \<omega>\<rangle> [\<Down>]\<^sub>t Val v'"
+| RedUnopFailure: "\<lbrakk> Pr, \<Delta>, \<omega>_def \<turnstile> \<langle>e; \<omega>\<rangle> [\<Down>]\<^sub>t VFailure \<rbrakk> \<Longrightarrow> Pr, \<Delta>, \<omega>_def \<turnstile> \<langle>Unop unop e; \<omega>\<rangle> [\<Down>]\<^sub>t VFailure" (* could be replaced *)
 
 \<comment>\<open>Cond\<close>
-| RedCondExpTrue: "\<lbrakk> Pr, \<Delta>, LH \<turnstile> \<langle>e1; \<omega>\<rangle> [\<Down>]\<^sub>t Val (VBool True) ; Pr, \<Delta>, LH \<turnstile> \<langle>e2; \<omega>\<rangle> [\<Down>]\<^sub>t r \<rbrakk>
-  \<Longrightarrow> Pr, \<Delta>, LH \<turnstile> \<langle>CondExp e1 e2 e3; \<omega>\<rangle> [\<Down>]\<^sub>t r"
-| RedCondExpFalse: "\<lbrakk> Pr, \<Delta>, LH \<turnstile> \<langle>e1; \<omega>\<rangle> [\<Down>]\<^sub>t Val (VBool False) ; Pr, \<Delta>, LH \<turnstile> \<langle>e3; \<omega>\<rangle> [\<Down>]\<^sub>t r \<rbrakk>
-  \<Longrightarrow> Pr, \<Delta>, LH \<turnstile> \<langle>CondExp e1 e2 e3; \<omega>\<rangle> [\<Down>]\<^sub>t r"
-| RedCondExpFailure: "\<lbrakk> Pr, \<Delta>, LH \<turnstile> \<langle>e1; \<omega>\<rangle> [\<Down>]\<^sub>t VFailure \<rbrakk>
-  \<Longrightarrow> Pr, \<Delta>, LH \<turnstile> \<langle>CondExp e1 e2 e3; \<omega>\<rangle> [\<Down>]\<^sub>t VFailure" (* could be replaced *)
+| RedCondExpTrue: "\<lbrakk> Pr, \<Delta>, \<omega>_def \<turnstile> \<langle>e1; \<omega>\<rangle> [\<Down>]\<^sub>t Val (VBool True) ; Pr, \<Delta>, \<omega>_def \<turnstile> \<langle>e2; \<omega>\<rangle> [\<Down>]\<^sub>t r \<rbrakk>
+  \<Longrightarrow> Pr, \<Delta>, \<omega>_def \<turnstile> \<langle>CondExp e1 e2 e3; \<omega>\<rangle> [\<Down>]\<^sub>t r"
+| RedCondExpFalse: "\<lbrakk> Pr, \<Delta>, \<omega>_def \<turnstile> \<langle>e1; \<omega>\<rangle> [\<Down>]\<^sub>t Val (VBool False) ; Pr, \<Delta>, \<omega>_def \<turnstile> \<langle>e3; \<omega>\<rangle> [\<Down>]\<^sub>t r \<rbrakk>
+  \<Longrightarrow> Pr, \<Delta>, \<omega>_def \<turnstile> \<langle>CondExp e1 e2 e3; \<omega>\<rangle> [\<Down>]\<^sub>t r"
+| RedCondExpFailure: "\<lbrakk> Pr, \<Delta>, \<omega>_def \<turnstile> \<langle>e1; \<omega>\<rangle> [\<Down>]\<^sub>t VFailure \<rbrakk>
+  \<Longrightarrow> Pr, \<Delta>, \<omega>_def \<turnstile> \<langle>CondExp e1 e2 e3; \<omega>\<rangle> [\<Down>]\<^sub>t VFailure" (* could be replaced *)
 
 \<comment>\<open>Old\<close>
-| RedOld: "\<lbrakk> t l = Some \<phi> ; Pr, \<Delta>, LH \<turnstile> \<langle>e; (\<sigma>, t, \<phi>)\<rangle> [\<Down>]\<^sub>t v \<rbrakk> \<Longrightarrow> Pr, \<Delta>, LH \<turnstile> \<langle>Old l e; (\<sigma>, t, _)\<rangle> [\<Down>]\<^sub>t v"
-| RedOldFailure: "\<lbrakk> t l = None \<rbrakk> \<Longrightarrow> Pr, \<Delta>, LH \<turnstile> \<langle>Old l e ; (_, t, _)\<rangle> [\<Down>]\<^sub>t VFailure" 
+| RedOld: "\<lbrakk> t l = Some \<phi> ; Pr, \<Delta>, \<omega>_def \<turnstile> \<langle>e; (\<sigma>, t, \<phi>)\<rangle> [\<Down>]\<^sub>t v \<rbrakk> \<Longrightarrow> Pr, \<Delta>, \<omega>_def \<turnstile> \<langle>Old l e; (\<sigma>, t, _)\<rangle> [\<Down>]\<^sub>t v"
+| RedOldFailure: "\<lbrakk> t l = None \<rbrakk> \<Longrightarrow> Pr, \<Delta>, \<omega>_def \<turnstile> \<langle>Old l e ; (_, t, _)\<rangle> [\<Down>]\<^sub>t VFailure" 
 
 \<comment>\<open>Heap lookup (TODO: null case?)\<close>
-| RedField: "\<lbrakk> Pr, \<Delta>, LH \<turnstile> \<langle>e; \<omega>\<rangle> [\<Down>]\<^sub>t Val (VRef (Address a)) ; get_hh_total_full \<omega> (a, f) = v \<rbrakk> \<Longrightarrow> 
-       Pr, \<Delta>, LH \<turnstile> \<langle>FieldAcc e f; \<omega>\<rangle> [\<Down>]\<^sub>t (if (a,f) \<in> LH then Val v else VFailure)"
-| RedFieldFailure: "\<lbrakk> Pr, \<Delta>, LH \<turnstile> \<langle>e; \<omega>\<rangle> [\<Down>]\<^sub>t VFailure \<rbrakk> \<Longrightarrow> Pr, \<Delta>, LH \<turnstile> \<langle>FieldAcc e f; \<omega>\<rangle> [\<Down>]\<^sub>t VFailure" (* could be replaced *)
+| RedField: "\<lbrakk> Pr, \<Delta>, \<omega>_def \<turnstile> \<langle>e; \<omega>\<rangle> [\<Down>]\<^sub>t Val (VRef (Address a)) ; get_hh_total_full \<omega> (a, f) = v \<rbrakk> \<Longrightarrow> 
+       Pr, \<Delta>, \<omega>_def \<turnstile> \<langle>FieldAcc e f; \<omega>\<rangle> [\<Down>]\<^sub>t (if (if_Some \<omega>_def (\<lambda>res. (a,f) \<in> get_valid_locs res)) then Val v else VFailure)"
+| RedFieldFailure: "\<lbrakk> Pr, \<Delta>, \<omega>_def \<turnstile> \<langle>e; \<omega>\<rangle> [\<Down>]\<^sub>t VFailure \<rbrakk> \<Longrightarrow> Pr, \<Delta>, \<omega>_def \<turnstile> \<langle>FieldAcc e f; \<omega>\<rangle> [\<Down>]\<^sub>t VFailure" (* could be replaced *)
 
 \<comment>\<open>Permission introspection\<close>
-| RedPermNull: "\<lbrakk> Pr, \<Delta>, LH \<turnstile> \<langle>e; \<omega>\<rangle> [\<Down>]\<^sub>t Val (VRef Null) \<rbrakk> \<Longrightarrow> Pr, \<Delta>, LH \<turnstile> \<langle>Perm e f; \<omega>\<rangle> [\<Down>]\<^sub>t Val (VPerm 0)"
-| RedPerm: "\<lbrakk> Pr, \<Delta>, LH \<turnstile> \<langle>e; \<omega>\<rangle> [\<Down>]\<^sub>t Val (VRef (Address a)) \<rbrakk> \<Longrightarrow> Pr, \<Delta>, LH \<turnstile> \<langle>Perm e f; \<omega>\<rangle> [\<Down>]\<^sub>t Val (VPerm (Rep_prat (get_mh_total_full \<omega> (a, f))))"
-| RedPermFailure: "\<lbrakk> Pr, \<Delta>, LH \<turnstile> \<langle>e; \<omega>\<rangle> [\<Down>]\<^sub>t VFailure \<rbrakk> \<Longrightarrow> Pr, \<Delta>, LH \<turnstile> \<langle>Perm e f; \<omega>\<rangle> [\<Down>]\<^sub>t VFailure" (* could be replaced *)
-(*
+| RedPermNull: "\<lbrakk> Pr, \<Delta>, \<omega>_def \<turnstile> \<langle>e; \<omega>\<rangle> [\<Down>]\<^sub>t Val (VRef Null) \<rbrakk> \<Longrightarrow> Pr, \<Delta>, \<omega>_def \<turnstile> \<langle>Perm e f; \<omega>\<rangle> [\<Down>]\<^sub>t Val (VPerm 0)"
+| RedPerm: "\<lbrakk> Pr, \<Delta>, \<omega>_def \<turnstile> \<langle>e; \<omega>\<rangle> [\<Down>]\<^sub>t Val (VRef (Address a)) \<rbrakk> \<Longrightarrow> Pr, \<Delta>, \<omega>_def \<turnstile> \<langle>Perm e f; \<omega>\<rangle> [\<Down>]\<^sub>t Val (VPerm (Rep_prat (get_mh_total_full \<omega> (a, f))))"
+| RedPermFailure: "\<lbrakk> Pr, \<Delta>, \<omega>_def \<turnstile> \<langle>e; \<omega>\<rangle> [\<Down>]\<^sub>t VFailure \<rbrakk> \<Longrightarrow> Pr, \<Delta>, \<omega>_def \<turnstile> \<langle>Perm e f; \<omega>\<rangle> [\<Down>]\<^sub>t VFailure" (* could be replaced *)
+
 \<comment>\<open>Unfolding\<close>
+| "\<lbrakk> Pr, \<Delta>, None \<turnstile> \<langle>ubody; \<omega>\<rangle> [\<Down>]\<^sub>t v \<rbrakk> \<Longrightarrow>   
+     Pr, \<Delta>, None \<turnstile> \<langle>Unfolding p es ubody; \<omega>\<rangle> [\<Down>]\<^sub>t v"
+| "\<lbrakk> red_pure_exps_total Pr \<Delta> (Some \<omega>_def) es \<omega> (Some vs);
+     unfold_rel Pr \<Delta> pred_id vs pwrite \<omega>_def \<omega>'_def;
+     Pr, \<Delta>, (Some \<omega>'_def) \<turnstile> \<langle>ubody; \<omega>\<rangle> [\<Down>]\<^sub>t v \<rbrakk> \<Longrightarrow>   
+     Pr, \<Delta>, (Some \<omega>_def) \<turnstile> \<langle>Unfolding p es ubody ; \<omega>\<rangle> [\<Down>]\<^sub>t v"
+(*                                                               
 | RedUnfolding: "\<lbrakk> 
          Pr, \<Delta>, LH \<turnstile> \<langle>e_arg; \<omega>\<rangle> [\<Down>]\<^sub>t v_arg;
         ViperLang.predicates Pr p = Some pred;
@@ -224,66 +244,62 @@ inductive red_pure_exp_total :: "program \<Rightarrow> 'a interp \<Rightarrow> h
 
 section \<open>Simplified induction principles\<close>
 lemma conj2conj2: "A \<and> B \<and> C \<Longrightarrow> C"
-  apply (rule conjunct2)
-  apply (erule conjunct2)
-  done
+  apply (drule conjunct2)
+  apply (drule conjunct2)
+  by assumption
 
-lemmas red_inhale_induct_aux = mp[OF conj2conj2[OF red_pure_exp_total_red_pure_exps_total_red_inhale.induct[where ?P1.0 = "\<lambda> a b c d. True" and ?P2.0 = "\<lambda> a b c d. True"]]]
+lemma conj2conj2conj1: "A \<and> B \<and> C \<and> D \<Longrightarrow> C"
+  apply (drule conjunct2)
+  apply (drule conjunct2)
+  apply (drule conjunct1)
+  by assumption
+
+
+lemmas red_inhale_induct_aux = mp[OF conj2conj2conj1[OF 
+      red_pure_exp_total_red_pure_exps_total_red_inhale_unfold_rel.induct[where ?P1.0 = "\<lambda> a b c d. True" and ?P2.0 = "\<lambda> a b c d. True" and ?P4.0 = "\<lambda> a b c d e. True"]]]
 
 lemma red_inhale_induct [consumes 1, case_names InhAcc InhAccPred InhAccWildcard InhAccPredWildcard 
 InhPureNormalMagic InhSubFailure InhSepNormal InhSepFailureMagic InhImpTrue InhImpFalse InhImpFailure]:
   assumes "red_inhale Pr \<Delta> R A \<omega> res" and
     "(\<And>\<omega> e_r r e_p p W' R f res.
-            Pr, \<Delta>, get_valid_locs \<omega> \<turnstile> \<langle>e_r;\<omega>\<rangle> [\<Down>]\<^sub>t Val (VRef r) \<Longrightarrow>
-            Pr, \<Delta>, get_valid_locs \<omega> \<turnstile> \<langle>e_p;\<omega>\<rangle> [\<Down>]\<^sub>t Val (VPerm p) \<Longrightarrow>
+            Pr, \<Delta>, (Some \<omega>) \<turnstile> \<langle>e_r;\<omega>\<rangle> [\<Down>]\<^sub>t Val (VRef r) \<Longrightarrow>
+            Pr, \<Delta>, (Some \<omega>) \<turnstile> \<langle>e_p;\<omega>\<rangle> [\<Down>]\<^sub>t Val (VPerm p) \<Longrightarrow>
             W' = inhale_perm_single R \<omega> (the_address r, f) (Some (Abs_prat p)) \<Longrightarrow>
             th_result_rel (0 \<le> p) (W' \<noteq> {} \<and> r \<noteq> Null) W' res \<Longrightarrow> P R (Atomic (Acc e_r f (PureExp e_p))) \<omega> res)" and
     "(\<And>\<omega> e_p p e_args v_args W' R pred_id res.
-            Pr, \<Delta>, get_valid_locs \<omega> \<turnstile> \<langle>e_p;\<omega>\<rangle> [\<Down>]\<^sub>t Val (VPerm p) \<Longrightarrow>
-            red_pure_exps_total Pr \<Delta> (get_valid_locs \<omega>) e_args \<omega> (Some v_args) \<Longrightarrow>
+            Pr, \<Delta>, (Some \<omega>) \<turnstile> \<langle>e_p;\<omega>\<rangle> [\<Down>]\<^sub>t Val (VPerm p) \<Longrightarrow>
+            red_pure_exps_total Pr \<Delta> (Some \<omega>) e_args \<omega> (Some v_args) \<Longrightarrow>
             W' = inhale_perm_single_pred R \<omega> (pred_id, v_args) (Some (Abs_prat p)) \<Longrightarrow>
             th_result_rel (0 \<le> p) (W' \<noteq> {}) W' res \<Longrightarrow> P R (Atomic (AccPredicate pred_id e_args (PureExp e_p))) \<omega> res)" and
     "(\<And>\<omega> e_r r W' R f res.
-            Pr, \<Delta>, get_valid_locs \<omega> \<turnstile> \<langle>e_r;\<omega>\<rangle> [\<Down>]\<^sub>t Val (VRef r) \<Longrightarrow>
+            Pr, \<Delta>, (Some \<omega>) \<turnstile> \<langle>e_r;\<omega>\<rangle> [\<Down>]\<^sub>t Val (VRef r) \<Longrightarrow>
             W' = inhale_perm_single R \<omega> (the_address r, f) None \<Longrightarrow>
             th_result_rel True (W' \<noteq> {} \<and> r \<noteq> Null) W' res \<Longrightarrow> P R (Atomic (Acc e_r f Wildcard)) \<omega> res)" and
     "(\<And>\<omega> e_args v_args W' R pred_id res.
-            red_pure_exps_total Pr \<Delta> (get_valid_locs \<omega>) e_args \<omega> (Some v_args) \<Longrightarrow>
+            red_pure_exps_total Pr \<Delta> (Some \<omega>) e_args \<omega> (Some v_args) \<Longrightarrow>
             W' = inhale_perm_single_pred R \<omega> (pred_id, v_args) None \<Longrightarrow>
             th_result_rel True (W' \<noteq> {}) W' res \<Longrightarrow> P R (Atomic (AccPredicate pred_id e_args Wildcard)) \<omega> res)"
     "(\<And>\<omega> e b R.
-            Pr, \<Delta>, get_valid_locs \<omega> \<turnstile> \<langle>e;\<omega>\<rangle> [\<Down>]\<^sub>t Val (VBool b) \<Longrightarrow>
+            Pr, \<Delta>, (Some \<omega>) \<turnstile> \<langle>e;\<omega>\<rangle> [\<Down>]\<^sub>t Val (VBool b) \<Longrightarrow>
             P R (Atomic (Pure e)) \<omega> (if b then RNormal \<omega> else RMagic))" and
     "(\<And>e A \<omega> R.
-            e \<in> sub_expressions_atomic A \<Longrightarrow> Pr, \<Delta>, get_valid_locs \<omega> \<turnstile> \<langle>e;\<omega>\<rangle> [\<Down>]\<^sub>t VFailure \<Longrightarrow> True \<Longrightarrow> P R (Atomic A) \<omega> RFailure)" and
+            e \<in> sub_expressions_atomic A \<Longrightarrow> Pr, \<Delta>, (Some \<omega>) \<turnstile> \<langle>e;\<omega>\<rangle> [\<Down>]\<^sub>t VFailure \<Longrightarrow> True \<Longrightarrow> P R (Atomic A) \<omega> RFailure)" and
     "(\<And>R A \<omega> \<omega>'' B res.
             red_inhale Pr \<Delta> R A \<omega> (RNormal \<omega>'') \<Longrightarrow>
             P R A \<omega> (RNormal \<omega>'') \<Longrightarrow> red_inhale Pr \<Delta> R B \<omega>'' res \<Longrightarrow> P R B \<omega>'' res \<Longrightarrow> P R (A && B) \<omega> res)" and
     "(\<And>R A \<omega> resA B. red_inhale Pr \<Delta> R A \<omega> resA \<Longrightarrow> P R A \<omega> resA \<Longrightarrow> resA = RFailure \<or> resA = RMagic \<Longrightarrow> P R (A && B) \<omega> resA)" and
     "(\<And>\<omega> e R A res.
-            Pr, \<Delta>, get_valid_locs \<omega> \<turnstile> \<langle>e;\<omega>\<rangle> [\<Down>]\<^sub>t Val (VBool True) \<Longrightarrow>
+            Pr, \<Delta>, (Some \<omega>) \<turnstile> \<langle>e;\<omega>\<rangle> [\<Down>]\<^sub>t Val (VBool True) \<Longrightarrow>
             red_inhale Pr \<Delta> R A \<omega> res \<Longrightarrow> P R A \<omega> res \<Longrightarrow> P R (Imp e A) \<omega> res)" and
-    "(\<And>\<omega> e R A. Pr, \<Delta>, get_valid_locs \<omega> \<turnstile> \<langle>e;\<omega>\<rangle> [\<Down>]\<^sub>t Val (VBool False) \<Longrightarrow> P R (Imp e A) \<omega> (RNormal \<omega>))" and
-    "(\<And>\<omega> e R A. Pr, \<Delta>, get_valid_locs \<omega> \<turnstile> \<langle>e;\<omega>\<rangle> [\<Down>]\<^sub>t VFailure \<Longrightarrow> P R (Imp e A) \<omega> RFailure)" and
-    "(\<And>\<omega> e R A. Pr, \<Delta>, get_valid_locs \<omega> \<turnstile> \<langle>e;\<omega>\<rangle> [\<Down>]\<^sub>t VFailure \<Longrightarrow> P R (Imp e A) \<omega> RFailure)"
+    "(\<And>\<omega> e R A. Pr, \<Delta>, (Some \<omega>) \<turnstile> \<langle>e;\<omega>\<rangle> [\<Down>]\<^sub>t Val (VBool False) \<Longrightarrow> P R (Imp e A) \<omega> (RNormal \<omega>))" and
+    "(\<And>\<omega> e R A. Pr, \<Delta>, (Some \<omega>) \<turnstile> \<langle>e;\<omega>\<rangle> [\<Down>]\<^sub>t VFailure \<Longrightarrow> P R (Imp e A) \<omega> RFailure)" and
+    "(\<And>\<omega> e R A. Pr, \<Delta>, (Some \<omega>) \<turnstile> \<langle>e;\<omega>\<rangle> [\<Down>]\<^sub>t VFailure \<Longrightarrow> P R (Imp e A) \<omega> RFailure)"
  shows "P R A \<omega> res"
   apply (rule red_inhale_induct_aux[where ?P3.0=P])
+  apply simp
   by (tactic \<open>resolve_tac @{context} @{thms assms} 1\<close>, assumption+)+ (auto intro: assms(1))
 
 section \<open>Total heap consistency\<close>
-
-inductive unfold_rel :: "program \<Rightarrow> 'a interp \<Rightarrow> predicate_ident \<Rightarrow> ('a val list) \<Rightarrow> prat \<Rightarrow> 'a full_total_state \<Rightarrow> 'a full_total_state \<Rightarrow> bool"
-  where 
-   UnfoldRelStep: 
-    "\<lbrakk> ViperLang.predicates Pr pred_id = Some pred_decl;
-     ViperLang.predicate_decl.body pred_decl = Some pred_body;
-     m = get_mp_total_full \<omega>;
-     pgte (m (pred_id,vs)) q;
-     q \<noteq> pnone;
-     m' = m( (pred_id,vs) := psub (m (pred_id, vs)) q);
-     \<omega>2 = (nth_option vs, get_trace_total \<omega>, update_mp_total (get_total_full \<omega>) m');
-     red_inhale Pr \<Delta> (\<lambda>_. True) (syntactic_mult (Rep_prat q) pred_body) \<omega>2 (RNormal \<omega>') \<rbrakk> \<Longrightarrow> 
-     unfold_rel Pr \<Delta> pred_id vs q \<omega> \<omega>'"
 
 definition unfold_rel_general :: "program \<Rightarrow> 'a interp \<Rightarrow> 'a full_total_state \<Rightarrow> 'a full_total_state \<Rightarrow> bool"
   where "unfold_rel_general Pr \<Delta> \<omega> \<omega>' \<equiv> \<exists> pred_id vs q. unfold_rel Pr \<Delta> pred_id vs q \<omega> \<omega>'"
@@ -296,10 +312,10 @@ e is well-defined and is deterministic (for example, if e is the body of a predi
 is used to indicate that every heap location can be read (effectively omitting heap checks)\<close>
 
 fun red_pure_exp_total_fun :: "program \<Rightarrow> 'a interp \<Rightarrow> pure_exp \<Rightarrow> 'a full_total_state \<Rightarrow> 'a val"
-  where "red_pure_exp_total_fun Pr \<Delta> e \<omega> = (SOME v. Pr, \<Delta>, UNIV \<turnstile> \<langle>e; \<omega>\<rangle> [\<Down>]\<^sub>t Val v)"
+  where "red_pure_exp_total_fun Pr \<Delta> e \<omega> = (SOME v. Pr, \<Delta>, None \<turnstile> \<langle>e; \<omega>\<rangle> [\<Down>]\<^sub>t Val v)"
 
 fun red_pure_exps_total_fun :: "program \<Rightarrow> 'a interp \<Rightarrow> pure_exp list \<Rightarrow> 'a full_total_state \<Rightarrow> ('a val) list"
-  where "red_pure_exps_total_fun Pr \<Delta> es \<omega> = (SOME vs. red_pure_exps_total Pr \<Delta> UNIV es \<omega> (Some vs))"
+  where "red_pure_exps_total_fun Pr \<Delta> es \<omega> = (SOME vs. red_pure_exps_total Pr \<Delta> None es \<omega> (Some vs))"
 
 (* TODO: duplicate? *)
 fun extract_address_from_val :: "'a val \<Rightarrow> address"
